better invariants for while loops

pulse/src/ml/PulseSyntaxExtension_SyntaxWrapper.ml
@@ -143,9 +143,11 @@ let tm_let_mut (x:binder) (v:term) (k:st_term) r : st_term =
 let tm_let_mut_array (x:binder) (v:term) (n:term) (k:st_term) (r:range) : st_term =
   PSB.(with_range (tm_with_local_array x v n k) r)
 
-  
 let tm_while (head:st_term) (invariant: (ident * slprop)) (body:st_term) r : st_term =
   PSB.(with_range (tm_while (snd invariant) head (ppname_of_id (fst invariant)) body) r)
+   
+let tm_nuwhile (head:st_term) (invariant: slprop) (body:st_term) r : st_term =
+  PSB.(with_range (tm_nuwhile invariant head body) r)
    
 let tm_if (head:term) (returns_annot:slprop option) (then_:st_term) (else_:st_term) r : st_term =
   PSB.(with_range (tm_if head then_ else_ returns_annot) r)
